rocq/theories/TypeSystem/CheckerSoundness.v
@@ -1,6 +1,10 @@
 From Facet.TypeSystem Require Import Types Syntax TypingRules TypeChecker.
-From Stdlib Require Import List String Bool Lia.
+From Stdlib Require Import List String Bool Lia PeanoNat Program.Equality.
 Import ListNotations.
+
+Scheme typed_ind' := Induction for typed Sort Prop
+with typed_args_ind' := Induction for typed_args Sort Prop.
+Combined Scheme typed_typed_args_ind from typed_ind', typed_args_ind'.
 
 (* ------------------------------------------------------------------ *)
 (* Auxiliary: usage_sub_bool correctness                                 *)
@@ -424,6 +428,16 @@ Proof.
   exact Halpha.
 Qed.
 
+Lemma ctx_alpha_remove_bound : forall ρ Γ Γr x xr,
+  ctx_alpha ((x, xr) :: ρ) Γ Γr ->
+  ctx_alpha ρ (ctx_remove x Γ) (ctx_remove xr Γr).
+Proof.
+  intros ρ Γ Γr x xr Halpha.
+  inversion Halpha; subst.
+  simpl. rewrite ident_eqb_refl. rewrite ident_eqb_refl.
+  assumption.
+Qed.
+
 Lemma ctx_alpha_is_ok_backward : forall ρ Γ Γr x T,
   ctx_alpha ρ Γ Γr ->
   ~ In x (rename_range ρ) ->
@@ -438,6 +452,118 @@ Proof.
   destruct b; try contradiction.
   rewrite (ctx_alpha_lookup_backward ρ Γ Γr x Tx true Halpha Hsafe Hlookup).
   exact I.
+Qed.
+
+Inductive ctx_same_bindings : ctx -> ctx -> Prop :=
+  | CtxSame_Nil :
+      ctx_same_bindings [] []
+  | CtxSame_Cons : forall x T b b' Γ Γ',
+      ctx_same_bindings Γ Γ' ->
+      ctx_same_bindings ((x, T, b) :: Γ) ((x, T, b') :: Γ').
+
+Lemma ctx_same_bindings_refl : forall Γ,
+  ctx_same_bindings Γ Γ.
+Proof.
+  induction Γ as [| [[x T] b] Γ IH].
+  - constructor.
+  - constructor. exact IH.
+Qed.
+
+Lemma ctx_same_bindings_names : forall Γ Γ',
+  ctx_same_bindings Γ Γ' ->
+  ctx_names Γ' = ctx_names Γ.
+Proof.
+  intros Γ Γ' Hsame.
+  induction Hsame; simpl; [reflexivity |].
+  rewrite IHHsame. reflexivity.
+Qed.
+
+Lemma ctx_same_bindings_trans : forall Γ1 Γ2 Γ3,
+  ctx_same_bindings Γ1 Γ2 ->
+  ctx_same_bindings Γ2 Γ3 ->
+  ctx_same_bindings Γ1 Γ3.
+Proof.
+  intros Γ1 Γ2 Γ3 H12 H23.
+  revert Γ3 H23.
+  induction H12 as [| x T b b' Γ Γ' H12 IH]; intros Γ3 H23.
+  - inversion H23; subst. constructor.
+  - inversion H23; subst. constructor.
+    match goal with
+    | Htail : ctx_same_bindings Γ' _ |- _ => eapply IH; exact Htail
+    end.
+Qed.
+
+Lemma ctx_consume_same_bindings : forall x Γ Γ',
+  ctx_consume x Γ = Some Γ' ->
+  ctx_same_bindings Γ Γ'.
+Proof.
+  intros x Γ. revert x.
+  induction Γ as [| [[n T] b] Γ IH]; intros x Γ' Hconsume.
+  - discriminate.
+  - simpl in Hconsume.
+    destruct (ident_eqb x n).
+    + injection Hconsume as <-. constructor. apply ctx_same_bindings_refl.
+    + destruct (ctx_consume x Γ) as [Γt |] eqn:Htail.
+      2: discriminate.
+      injection Hconsume as <-.
+      constructor. eapply IH. exact Htail.
+Qed.
+
+Lemma ctx_remove_same_bindings_head : forall x T b b' Γ Γ',
+  ctx_same_bindings Γ Γ' ->
+  ctx_remove x ((x, T, b) :: Γ) = Γ ->
+  ctx_remove x ((x, T, b') :: Γ') = Γ'.
+Proof.
+  intros x T b b' Γ Γ' _ _.
+  simpl. rewrite ident_eqb_refl. reflexivity.
+Qed.
+
+Lemma ctx_same_bindings_remove_head : forall x T b Γ Γ',
+  ctx_same_bindings ((x, T, b) :: Γ) Γ' ->
+  ctx_same_bindings Γ (ctx_remove x Γ').
+Proof.
+  intros x T b Γ Γ' Hsame.
+  inversion Hsame; subst.
+  simpl. rewrite ident_eqb_refl. assumption.
+Qed.
+
+Lemma typed_same_bindings :
+  (forall fenv Γ e T Γ',
+      typed fenv Γ e T Γ' ->
+      ctx_same_bindings Γ Γ') /\
+  (forall fenv Γ es ps Γ',
+      typed_args fenv Γ es ps Γ' ->
+      ctx_same_bindings Γ Γ').
+Proof.
+  assert (H : forall fenv,
+    (forall Γ e T Γ',
+        typed fenv Γ e T Γ' -> ctx_same_bindings Γ Γ') /\
+    (forall Γ es ps Γ',
+        typed_args fenv Γ es ps Γ' -> ctx_same_bindings Γ Γ')).
+  {
+    intro fenv.
+    apply typed_typed_args_ind; intros; simpl;
+      try solve [apply ctx_same_bindings_refl];
+      try solve [eassumption];
+      try solve [
+        match goal with
+        | Hconsume : ctx_consume _ _ = Some _ |- _ =>
+            eapply ctx_consume_same_bindings; exact Hconsume
+        end
+      ];
+      try solve [
+        match goal with
+        | Hhead : ctx_same_bindings ?Γ ?Γ1,
+          Hbody : ctx_same_bindings (ctx_add ?x ?T ?Γ1) ?Γ2
+          |- ctx_same_bindings ?Γ (ctx_remove ?x ?Γ2) =>
+            eapply ctx_same_bindings_trans;
+            [ exact Hhead
+            | eapply ctx_same_bindings_remove_head; exact Hbody ]
+        end
+      ];
+      try solve [eapply ctx_same_bindings_trans; eassumption].
+  }
+  split; intros fenv; destruct (H fenv) as [Ht Hargs]; [apply Ht | apply Hargs].
 Qed.
 
 Fixpoint expr_size (e : expr) : nat :=
@@ -467,6 +593,191 @@ Proof.
   - simpl in *. destruct Hin as [<- | Hin].
     + lia.
     + specialize (IH arg Hin). simpl in IH. lia.
+Qed.
+
+Lemma alpha_rename_call_args_used_extends : forall ρ used args argsr used',
+  (forall used0 e er used1,
+      In e args ->
+      alpha_rename_expr ρ used0 e = (er, used1) ->
+      forall x, In x used0 -> In x used1) ->
+  ((fix go (used0 : list ident) (args0 : list expr)
+      : list expr * list ident :=
+      match args0 with
+      | [] => ([], used0)
+      | arg :: rest =>
+          let (arg', used1) := alpha_rename_expr ρ used0 arg in
+          let (rest', used2) := go used1 rest in
+          (arg' :: rest', used2)
+      end) used args) = (argsr, used') ->
+  forall x, In x used -> In x used'.
+Proof.
+  intros ρ used args.
+  revert used.
+  induction args as [| arg rest IH]; intros used argsr used' Hexpr Hrename x Hin;
+    simpl in Hrename.
+  - injection Hrename as _ <-. exact Hin.
+  - destruct (alpha_rename_expr ρ used arg) as [ar used1] eqn:Harg.
+    destruct ((fix go (used0 : list ident) (args0 : list expr)
+          : list expr * list ident :=
+          match args0 with
+          | [] => ([], used0)
+          | arg0 :: rest0 =>
+              let (arg', used2) := alpha_rename_expr ρ used0 arg0 in
+              let (rest', used3) := go used2 rest0 in
+              (arg' :: rest', used3)
+          end) used1 rest) as [restr used2] eqn:Hrest.
+    injection Hrename as _ <-.
+    eapply IH.
+    + intros used0 e er0 used_tail Hin_rest Hrename0.
+      eapply Hexpr.
+      * right. exact Hin_rest.
+      * exact Hrename0.
+    + exact Hrest.
+    + eapply Hexpr.
+      * left. reflexivity.
+      * exact Harg.
+      * exact Hin.
+Qed.
+
+Lemma alpha_rename_expr_used_extends : forall ρ used e er used',
+  alpha_rename_expr ρ used e = (er, used') ->
+  forall x, In x used -> In x used'.
+Proof.
+  assert (Hsize : forall n ρ used e er used',
+    expr_size e < n ->
+    alpha_rename_expr ρ used e = (er, used') ->
+    forall x, In x used -> In x used').
+  {
+  induction n as [| n IH]; intros ρ used e er used' Hlt Hrename x0 Hin.
+  - lia.
+  - destruct e; simpl in Hrename.
+  + injection Hrename as _ <-. exact Hin.
+  + injection Hrename as _ <-. exact Hin.
+  + injection Hrename as _ <-. exact Hin.
+  + destruct (alpha_rename_expr ρ used e1) as [e1r used1] eqn:He1.
+    destruct (alpha_rename_expr
+      ((i, fresh_ident i (i :: free_vars_expr e2 ++ used1)) :: ρ)
+      (fresh_ident i (i :: free_vars_expr e2 ++ used1) ::
+       i :: free_vars_expr e2 ++ used1) e2)
+      as [e2r used2] eqn:He2.
+    injection Hrename as _ <-.
+    eapply IH.
+    * simpl in Hlt. assert (expr_size e2 < n) as Hlt_e2 by lia. exact Hlt_e2.
+    * exact He2.
+    * right. right. apply in_or_app. right.
+      eapply IH.
+      -- simpl in Hlt. assert (expr_size e1 < n) as Hlt_e1 by lia. exact Hlt_e1.
+      -- exact He1.
+      -- exact Hin.
+  + destruct (alpha_rename_expr ρ used e1) as [e1r used1] eqn:He1.
+    destruct (alpha_rename_expr
+      ((i, fresh_ident i (i :: free_vars_expr e2 ++ used1)) :: ρ)
+      (fresh_ident i (i :: free_vars_expr e2 ++ used1) ::
+       i :: free_vars_expr e2 ++ used1) e2)
+      as [e2r used2] eqn:He2.
+    injection Hrename as _ <-.
+    eapply IH.
+    * simpl in Hlt. assert (expr_size e2 < n) as Hlt_e2 by lia. exact Hlt_e2.
+    * exact He2.
+    * right. right. apply in_or_app. right.
+      eapply IH.
+      -- simpl in Hlt. assert (expr_size e1 < n) as Hlt_e1 by lia. exact Hlt_e1.
+      -- exact He1.
+      -- exact Hin.
+  + remember
+      ((fix go (used0 : list ident) (args0 : list expr)
+          : list expr * list ident :=
+          match args0 with
+          | [] => ([], used0)
+          | arg :: rest =>
+              let (arg', used1) := alpha_rename_expr ρ used0 arg in
+              let (rest', used2) := go used1 rest in
+              (arg' :: rest', used2)
+          end) used l) as r eqn:Hargs.
+    destruct r as [argsr used_args].
+    injection Hrename as _ <-.
+    eapply alpha_rename_call_args_used_extends.
+    * intros used0 e er0 used1 Hin_arg Hrename0.
+      eapply IH.
+      -- pose proof (expr_size_call_arg_lt i l e Hin_arg) as Harg_lt.
+        assert (expr_size e < n) as Hlt_arg by lia.
+        exact Hlt_arg.
+      -- exact Hrename0.
+    * symmetry. exact Hargs.
+    * exact Hin.
+  + destruct (alpha_rename_expr ρ used e) as [er0 used0] eqn:He.
+    injection Hrename as _ <-.
+    eapply IH.
+    * simpl in Hlt. assert (expr_size e < n) as Hlt_e by lia. exact Hlt_e.
+    * exact He.
+    * exact Hin.
+  + destruct (alpha_rename_expr ρ used e) as [er0 used0] eqn:He.
+    injection Hrename as _ <-.
+    eapply IH.
+    * simpl in Hlt. assert (expr_size e < n) as Hlt_e by lia. exact Hlt_e.
+    * exact He.
+    * exact Hin.
+  }
+  intros ρ used e er used' Hrename x Hin.
+  eapply (Hsize (S (expr_size e))).
+  - apply Nat.lt_succ_diag_r.
+  - exact Hrename.
+  - exact Hin.
+Qed.
+
+Lemma alpha_rename_params_used_extends : forall ρ used ps psr ρ' used',
+  alpha_rename_params ρ used ps = (psr, ρ', used') ->
+  forall x, In x used -> In x used'.
+Proof.
+  intros ρ used ps.
+  revert ρ used.
+  induction ps as [| p ps IH]; intros ρ used psr ρ' used' Hrename x Hin.
+  - simpl in Hrename. injection Hrename as _ _ <-. exact Hin.
+  - simpl in Hrename.
+    destruct (alpha_rename_params
+      ((param_name p, fresh_ident (param_name p) used) :: ρ)
+      (fresh_ident (param_name p) used :: used) ps)
+      as [[ps0 ρ0] used0] eqn:Hps.
+    injection Hrename as _ _ <-.
+    eapply IH.
+    + exact Hps.
+    + right. exact Hin.
+Qed.
+
+Lemma alpha_rename_fn_def_used_extends : forall used f fr used',
+  alpha_rename_fn_def used f = (fr, used') ->
+  forall x, In x used -> In x used'.
+Proof.
+  intros used f fr used' Hrename x Hin.
+  destruct f as [fname ps ret body].
+  unfold alpha_rename_fn_def in Hrename. simpl in Hrename.
+  destruct (alpha_rename_params []
+    (param_names ps ++ free_vars_expr body ++ used) ps)
+    as [[psr ρ] used1] eqn:Hps.
+  destruct (alpha_rename_expr ρ used1 body) as [bodyr used2] eqn:Hbody.
+  injection Hrename as _ <-.
+  eapply alpha_rename_expr_used_extends.
+  - exact Hbody.
+  - eapply alpha_rename_params_used_extends.
+    + exact Hps.
+    + apply in_or_app. right. apply in_or_app. right. exact Hin.
+Qed.
+
+Lemma alpha_rename_syntax_go_used_extends : forall used fenv fenvr used',
+  alpha_rename_syntax_go used fenv = (fenvr, used') ->
+  forall x, In x used -> In x used'.
+Proof.
+  intros used fenv.
+  revert used.
+  induction fenv as [| f fs IH]; intros used fenvr used' Hrename x Hin.
+  - simpl in Hrename. injection Hrename as _ <-. exact Hin.
+  - simpl in Hrename.
+    destruct (alpha_rename_fn_def used f) as [fr used1] eqn:Hf.
+    destruct (alpha_rename_syntax_go used1 fs) as [fsr used2] eqn:Hfs.
+    injection Hrename as _ <-.
+    eapply IH.
+    + exact Hfs.
+    + eapply alpha_rename_fn_def_used_extends; [exact Hf | exact Hin].
 Qed.
 
 Lemma alpha_rename_call_args_sound : forall ρ used args argsr used',
@@ -553,9 +864,9 @@ Proof.
     { intros x Hin. apply Hdisj. simpl. right. exact Hin. }
     destruct (alpha_rename_expr ρ used e1) as [e1r used1] eqn:He1.
     destruct (alpha_rename_expr
-      ((i, fresh_ident i (free_vars_expr e2 ++ used1)) :: ρ)
-      (fresh_ident i (free_vars_expr e2 ++ used1) ::
-       free_vars_expr e2 ++ used1) e2)
+      ((i, fresh_ident i (i :: free_vars_expr e2 ++ used1)) :: ρ)
+      (fresh_ident i (i :: free_vars_expr e2 ++ used1) ::
+       i :: free_vars_expr e2 ++ used1) e2)
       as [e2r used2] eqn:He2.
     injection Hrename as <- _.
     constructor.
@@ -568,8 +879,8 @@ Proof.
       -- intros x Hin.
         simpl. intros [Heq | Hin_range].
         ++ subst x.
-           apply (fresh_ident_not_in i (free_vars_expr e2 ++ used1)).
-           apply in_or_app. left. exact Hin.
+           apply (fresh_ident_not_in i (i :: free_vars_expr e2 ++ used1)).
+           right. apply in_or_app. left. exact Hin.
         ++ exact (Hdisj2 x Hin Hin_range).
       -- exact He2.
   + destruct (disjoint_names_app_l (free_vars_expr e1) (free_vars_expr e2)
@@ -577,9 +888,9 @@ Proof.
     { intros x Hin. apply Hdisj. simpl. right. exact Hin. }
     destruct (alpha_rename_expr ρ used e1) as [e1r used1] eqn:He1.
     destruct (alpha_rename_expr
-      ((i, fresh_ident i (free_vars_expr e2 ++ used1)) :: ρ)
-      (fresh_ident i (free_vars_expr e2 ++ used1) ::
-       free_vars_expr e2 ++ used1) e2)
+      ((i, fresh_ident i (i :: free_vars_expr e2 ++ used1)) :: ρ)
+      (fresh_ident i (i :: free_vars_expr e2 ++ used1) ::
+       i :: free_vars_expr e2 ++ used1) e2)
       as [e2r used2] eqn:He2.
     injection Hrename as <- _.
     constructor.
@@ -592,8 +903,8 @@ Proof.
       -- intros x Hin.
         simpl. intros [Heq | Hin_range].
         ++ subst x.
-           apply (fresh_ident_not_in i (free_vars_expr e2 ++ used1)).
-           apply in_or_app. left. exact Hin.
+           apply (fresh_ident_not_in i (i :: free_vars_expr e2 ++ used1)).
+           right. apply in_or_app. left. exact Hin.
         ++ exact (Hdisj2 x Hin Hin_range).
       -- exact He2.
   + remember
@@ -715,28 +1026,432 @@ Proof.
     + exact He.
 Qed.
 
-Lemma typed_alpha_backward :
-  (forall fenv Γ e T Γr,
-      typed fenv Γ e T Γr ->
-      forall fenv0 ρ Γ0 e0,
-        fenv_alpha fenv0 fenv ->
-        ctx_alpha ρ Γ0 Γ ->
-        expr_alpha ρ e0 e ->
-        exists Γ0',
-          typed fenv0 Γ0 e0 T Γ0' /\
-          ctx_alpha ρ Γ0' Γr) /\
-  (forall fenv Γ es ps Γr,
-      typed_args fenv Γ es ps Γr ->
-      forall fenv0 ρ Γ0 es0 ps0,
-        fenv_alpha fenv0 fenv ->
-        ctx_alpha ρ Γ0 Γ ->
-        exprs_alpha ρ es0 es ->
-        params_alpha ps0 ps ->
-        exists Γ0',
-          typed_args fenv0 Γ0 es0 ps0 Γ0' /\
-          ctx_alpha ρ Γ0' Γr).
+Lemma params_alpha_cons_inv : forall ps0 pr psr,
+  params_alpha ps0 (pr :: psr) ->
+  exists p ps,
+    ps0 = p :: ps /\
+    same_param_shape p pr /\
+    params_alpha ps psr.
 Proof.
-Admitted.
+  intros ps0 pr psr Halpha.
+  inversion Halpha; subst.
+  exists p, ps.
+  split; [reflexivity |].
+  split; assumption.
+Qed.
+
+Lemma typed_args_cons_inv : forall fenv Γ er ers pr psr Γ',
+  typed_args fenv Γ (er :: ers) (pr :: psr) Γ' ->
+  exists T Γ1,
+    typed fenv Γ er T Γ1 /\
+    ty_core T = ty_core (param_ty pr) /\
+    usage_sub (ty_usage T) (ty_usage (param_ty pr)) /\
+    typed_args fenv Γ1 ers psr Γ'.
+Proof.
+  intros fenv Γ er ers pr psr Γ' Htyped.
+  inversion Htyped; subst.
+  exists T_e, Γ1. repeat split; assumption.
+Qed.
+
+Lemma typed_call_inv : forall fenv Γ fname args T Γ',
+  typed fenv Γ (ECall fname args) T Γ' ->
+  exists fdef,
+    In fdef fenv /\
+    fn_name fdef = fname /\
+    fn_ret fdef = T /\
+    typed_args fenv Γ args (fn_params fdef) Γ'.
+Proof.
+  intros fenv Γ fname args T Γ' Htyped.
+  inversion Htyped; subst.
+  exists fdef. repeat split; assumption.
+Qed.
+
+Lemma alpha_rename_call_args_typed_backward : forall fenv0 fenvr ρ Γ0 Γr args argsr used used' ps0 psr Γr',
+  (forall Γa Γb used0 e er used1 T Γb',
+      In e args ->
+      ctx_alpha ρ Γa Γb ->
+      (forall x, In x (ctx_names Γb) -> In x used0) ->
+      (forall x, In x (rename_range ρ) -> In x used0) ->
+      disjoint_names (free_vars_expr e) (rename_range ρ) ->
+      alpha_rename_expr ρ used0 e = (er, used1) ->
+      typed fenvr Γb er T Γb' ->
+      exists Γa',
+        typed fenv0 Γa e T Γa' /\
+        ctx_alpha ρ Γa' Γb') ->
+  fenv_alpha fenv0 fenvr ->
+  ctx_alpha ρ Γ0 Γr ->
+  (forall x, In x (ctx_names Γr) -> In x used) ->
+  (forall x, In x (rename_range ρ) -> In x used) ->
+  disjoint_names
+    ((fix go (args0 : list expr) : list ident :=
+        match args0 with
+        | [] => []
+        | arg :: rest => free_vars_expr arg ++ go rest
+        end) args)
+    (rename_range ρ) ->
+  params_alpha ps0 psr ->
+  ((fix go (used0 : list ident) (args0 : list expr)
+      : list expr * list ident :=
+      match args0 with
+      | [] => ([], used0)
+      | arg :: rest =>
+          let (arg', used1) := alpha_rename_expr ρ used0 arg in
+          let (rest', used2) := go used1 rest in
+          (arg' :: rest', used2)
+      end) used args) = (argsr, used') ->
+  typed_args fenvr Γr argsr psr Γr' ->
+  exists Γ0',
+    typed_args fenv0 Γ0 args ps0 Γ0' /\
+    ctx_alpha ρ Γ0' Γr'.
+Proof.
+  intros fenv0 fenvr ρ Γ0 Γr args.
+  revert Γ0 Γr.
+  induction args as [| arg rest IH]; intros Γ0 Γr argsr used used' ps0 psr Γr'
+    Hexpr Hfenv Hctx Hctx_used Hrange_used Hdisj Hparams Hrename Htyped_args;
+    simpl in Hrename.
+  - injection Hrename as <- <-.
+    inversion Htyped_args; subst.
+    inversion Hparams; subst.
+    exists Γ0. split; [constructor | exact Hctx].
+  - destruct (disjoint_names_app_l (free_vars_expr arg)
+      ((fix go (args0 : list expr) : list ident :=
+          match args0 with
+          | [] => []
+          | arg0 :: rest0 => free_vars_expr arg0 ++ go rest0
+          end) rest) (rename_range ρ) Hdisj) as [Hdisj_arg Hdisj_rest].
+    destruct (alpha_rename_expr ρ used arg) as [ar used1] eqn:Harg.
+    destruct ((fix go (used0 : list ident) (args0 : list expr)
+          : list expr * list ident :=
+          match args0 with
+          | [] => ([], used0)
+          | arg0 :: rest0 =>
+              let (arg', used2) := alpha_rename_expr ρ used0 arg0 in
+              let (rest', used3) := go used2 rest0 in
+              (arg' :: rest', used3)
+          end) used1 rest) as [restr used2] eqn:Hrest.
+    injection Hrename as <- <-.
+    destruct psr as [| pr psr_tail].
+    { inversion Htyped_args. }
+    destruct (params_alpha_cons_inv ps0 pr psr_tail Hparams)
+      as [p [ps [Hps0 [Hshape Hparams_tail]]]].
+    subst ps0.
+    destruct (typed_args_cons_inv fenvr Γr ar restr pr psr_tail Γr' Htyped_args)
+      as [Targ [Γr1 [Htyped_arg_r [Hcore [Hsub Htyped_tail_r]]]]].
+    destruct (Hexpr Γ0 Γr used arg ar used1 Targ Γr1)
+      as [Γ01 [Htyped_arg Hctx_arg]].
+    + left. reflexivity.
+    + exact Hctx.
+    + exact Hctx_used.
+    + exact Hrange_used.
+    + exact Hdisj_arg.
+    + exact Harg.
+    + exact Htyped_arg_r.
+    + assert (Hctx_used_tail : forall x, In x (ctx_names Γr1) -> In x used1).
+      { intros x Hin.
+        eapply alpha_rename_expr_used_extends.
+        - exact Harg.
+        - apply Hctx_used.
+          rewrite <- (ctx_same_bindings_names Γr Γr1).
+          + exact Hin.
+          + destruct typed_same_bindings as [Hsame _].
+            eapply Hsame. exact Htyped_arg_r. }
+      assert (Hrange_used_tail : forall x, In x (rename_range ρ) -> In x used1).
+      { intros x Hin.
+        eapply alpha_rename_expr_used_extends.
+        - exact Harg.
+        - apply Hrange_used. exact Hin. }
+      destruct (IH Γ01 Γr1 restr used1 used2 ps psr_tail Γr')
+        as [Γ02 [Htyped_tail Hctx_tail]].
+      * intros Γa Γb used0 e er used_tail T Γb' Hin Halpha Hcu Hru Hd Hr Ht.
+        eapply Hexpr.
+        -- right. exact Hin.
+        -- exact Halpha.
+        -- exact Hcu.
+        -- exact Hru.
+        -- exact Hd.
+        -- exact Hr.
+        -- exact Ht.
+      * exact Hfenv.
+      * exact Hctx_arg.
+      * exact Hctx_used_tail.
+      * exact Hrange_used_tail.
+      * exact Hdisj_rest.
+      * exact Hparams_tail.
+      * exact Hrest.
+      * exact Htyped_tail_r.
+      * exists Γ02. split.
+        -- eapply TArgs_Cons.
+           ++ exact Htyped_arg.
+           ++ destruct Hshape as [_ HT]. simpl in HT. rewrite HT. exact Hcore.
+           ++ destruct Hshape as [_ HT]. simpl in HT. rewrite HT. exact Hsub.
+           ++ exact Htyped_tail.
+        -- exact Hctx_tail.
+Qed.
+
+Lemma alpha_rename_typed_backward : forall fenv0 fenvr ρ Γ0 Γr e er used used' T Γr',
+  fenv_alpha fenv0 fenvr ->
+  ctx_alpha ρ Γ0 Γr ->
+  (forall x, In x (ctx_names Γr) -> In x used) ->
+  (forall x, In x (rename_range ρ) -> In x used) ->
+  disjoint_names (free_vars_expr e) (rename_range ρ) ->
+  alpha_rename_expr ρ used e = (er, used') ->
+  typed fenvr Γr er T Γr' ->
+  exists Γ0',
+    typed fenv0 Γ0 e T Γ0' /\
+    ctx_alpha ρ Γ0' Γr'.
+Proof.
+  assert (Hsize : forall n fenv0 fenvr ρ Γ0 Γr e er used used' T Γr',
+    expr_size e < n ->
+    fenv_alpha fenv0 fenvr ->
+    ctx_alpha ρ Γ0 Γr ->
+    (forall x, In x (ctx_names Γr) -> In x used) ->
+    (forall x, In x (rename_range ρ) -> In x used) ->
+    disjoint_names (free_vars_expr e) (rename_range ρ) ->
+    alpha_rename_expr ρ used e = (er, used') ->
+    typed fenvr Γr er T Γr' ->
+    exists Γ0',
+      typed fenv0 Γ0 e T Γ0' /\
+      ctx_alpha ρ Γ0' Γr').
+  {
+  induction n as [| n IH]; intros fenv0 fenvr ρ Γ0 Γr e er used used' T Γr'
+    Hlt Hfenv Hctx Hctx_used Hrange_used Hdisj Hrename Htyped.
+  - lia.
+  - destruct e; simpl in Hrename.
+  + injection Hrename as <- _.
+    inversion Htyped; subst.
+    eexists. split; [constructor | exact Hctx].
+  + injection Hrename as <- _.
+    inversion Htyped; subst.
+    * exists Γ0. split; [constructor | exact Hctx].
+    * exists Γ0. split; [constructor | exact Hctx].
+  + injection Hrename as <- _.
+    inversion Htyped; subst.
+    * assert (Hsafe : ~ In i (rename_range ρ)).
+      { intros Hin. apply (Hdisj i); simpl; [left; reflexivity | exact Hin]. }
+      lazymatch goal with
+      | Hlookup : ctx_lookup (lookup_rename i ρ) Γr = Some (T, false),
+        Hconsume_r : ctx_consume (lookup_rename i ρ) Γr = Some ?Γr1 |- _ =>
+      destruct (ctx_alpha_consume_backward ρ Γ0 Γr i Γr1 Hctx Hsafe Hconsume_r)
+        as [Γ0' [Hconsume Hctx']]
+      end.
+	      exists Γ0'. split.
+	      { eapply T_Var_Consume.
+	        - lazymatch goal with
+	          | Hlookup : ctx_lookup (lookup_rename i ρ) Γr = Some (T, false) |- _ =>
+	              exact (ctx_alpha_lookup_backward ρ Γ0 Γr i T false Hctx Hsafe Hlookup)
+	          end.
+	        - assumption.
+	        - exact Hconsume. }
+	      { exact Hctx'. }
+    * assert (Hsafe : ~ In i (rename_range ρ)).
+      { intros Hin. apply (Hdisj i); simpl; [left; reflexivity | exact Hin]. }
+	      exists Γ0. split.
+	      { eapply T_Var_Copy.
+	        - lazymatch goal with
+	          | Hlookup : ctx_lookup (lookup_rename i ρ) ?Γrx = Some (T, b),
+	            Halpha : ctx_alpha ρ Γ0 ?Γrx |- _ =>
+	              exact (ctx_alpha_lookup_backward ρ Γ0 Γrx i T b Halpha Hsafe Hlookup)
+	          end.
+	        - assumption. }
+	      { exact Hctx. }
+  + destruct (alpha_rename_expr ρ used e1) as [e1r used1] eqn:He1.
+    destruct (alpha_rename_expr
+      ((i, fresh_ident i (i :: free_vars_expr e2 ++ used1)) :: ρ)
+      (fresh_ident i (i :: free_vars_expr e2 ++ used1) ::
+       i :: free_vars_expr e2 ++ used1) e2)
+      as [e2r used2] eqn:He2.
+    injection Hrename as <- _.
+    inversion Htyped; subst.
+    destruct (disjoint_names_app_l (free_vars_expr e1) (free_vars_expr e2)
+      (rename_range ρ)) as [Hdisj1 Hdisj2].
+    { intros x Hin. apply Hdisj. simpl. right. exact Hin. }
+    lazymatch goal with
+    | Hte1 : typed fenvr Γr e1r ?T1r ?Γ1r |- _ =>
+      destruct (IH fenv0 fenvr ρ Γ0 Γr e1 e1r used used1 T1r Γ1r
+        ltac:(simpl in Hlt; lia)
+        Hfenv Hctx Hctx_used Hrange_used Hdisj1 He1 Hte1)
+        as [Γ01 [Htyped1 Hctx1]]
+    end.
+    set (xr := fresh_ident i (i :: free_vars_expr e2 ++ used1)).
+    assert (Hctx1_names : forall x, In x (ctx_names Γ1) -> In x used1).
+    { intros x Hin.
+      eapply alpha_rename_expr_used_extends.
+      - exact He1.
+      - apply Hctx_used.
+        rewrite <- (ctx_same_bindings_names Γr Γ1).
+        + exact Hin.
+        + destruct typed_same_bindings as [Hsame _].
+          lazymatch goal with
+          | Hte1 : typed fenvr Γr e1r _ _ |- _ => eapply Hsame; exact Hte1
+          end. }
+    assert (Hxr_ctx : ~ In xr (ctx_names Γ1)).
+    { unfold xr. intros Hin.
+      apply (fresh_ident_not_in i (i :: free_vars_expr e2 ++ used1)).
+      right. apply in_or_app. right. apply Hctx1_names. exact Hin. }
+    assert (Hxr_range : ~ In xr (rename_range ρ)).
+    { unfold xr. intros Hin.
+      apply (fresh_ident_not_in i (i :: free_vars_expr e2 ++ used1)).
+      right. apply in_or_app. right.
+      eapply alpha_rename_expr_used_extends.
+      - exact He1.
+      - apply Hrange_used. exact Hin. }
+    assert (Hctx_ext :
+      ctx_alpha ((i, xr) :: ρ)
+        (ctx_add i t Γ01) (ctx_add xr t Γ1)).
+    { constructor; exact Hctx1 || exact Hxr_ctx || exact Hxr_range. }
+    assert (Hctx_ext_used :
+      forall x, In x (ctx_names (ctx_add xr t Γ1)) ->
+        In x (xr :: i :: free_vars_expr e2 ++ used1)).
+    { intros x [Hx | Hin]; [left; exact Hx |].
+      right. right. apply in_or_app. right. apply Hctx1_names. exact Hin. }
+    assert (Hrange_ext_used :
+      forall x, In x (rename_range ((i, xr) :: ρ)) ->
+        In x (xr :: i :: free_vars_expr e2 ++ used1)).
+    { intros x [Hx | Hin]; [left; exact Hx |].
+      right. right. apply in_or_app. right.
+      eapply alpha_rename_expr_used_extends.
+      - exact He1.
+      - apply Hrange_used. exact Hin. }
+    assert (Hdisj2_ext :
+      disjoint_names (free_vars_expr e2) (rename_range ((i, xr) :: ρ))).
+    { intros x Hin [Hx | Hinr].
+      - subst x. unfold xr in *.
+        apply (fresh_ident_not_in i (i :: free_vars_expr e2 ++ used1)).
+        right. apply in_or_app. left. exact Hin.
+      - exact (Hdisj2 x Hin Hinr). }
+    lazymatch goal with
+    | Hte2 : typed fenvr (ctx_add ?xrr t Γ1) e2r ?T2r ?Γ2r |- _ =>
+      destruct (IH fenv0 fenvr ((i, xr) :: ρ)
+        (ctx_add i t Γ01) (ctx_add xrr t Γ1)
+        e2 e2r (xr :: i :: free_vars_expr e2 ++ used1) used2 T2r Γ2r
+        ltac:(simpl in Hlt; lia)
+        Hfenv Hctx_ext Hctx_ext_used Hrange_ext_used Hdisj2_ext He2 Hte2)
+        as [Γ02 [Htyped2 Hctx2]]
+    end.
+	    exists (ctx_remove i Γ02). split.
+	    { eapply T_Let.
+	      - exact Htyped1.
+	      - assumption.
+	      - assumption.
+	      - exact Htyped2.
+	      - eapply ctx_alpha_is_ok_backward.
+	        + exact Hctx2.
+	        + simpl. intros [Heq | Hinr].
+	          * apply (fresh_ident_not_in i (i :: free_vars_expr e2 ++ used1)).
+	            fold xr. rewrite Heq. left. reflexivity.
+	          * apply (Hdisj i); simpl; [left; reflexivity | exact Hinr].
+	        + simpl. rewrite ident_eqb_refl. exact H11. }
+	    { eapply ctx_alpha_remove_bound. exact Hctx2. }
+  + destruct (alpha_rename_expr ρ used e1) as [e1r used1] eqn:He1.
+    destruct (alpha_rename_expr
+      ((i, fresh_ident i (i :: free_vars_expr e2 ++ used1)) :: ρ)
+      (fresh_ident i (i :: free_vars_expr e2 ++ used1) ::
+       i :: free_vars_expr e2 ++ used1) e2)
+      as [e2r used2] eqn:He2.
+    injection Hrename as <- _.
+    inversion Htyped.
+  + remember
+      ((fix go (used0 : list ident) (args0 : list expr)
+          : list expr * list ident :=
+          match args0 with
+          | [] => ([], used0)
+          | arg :: rest =>
+              let (arg', used1) := alpha_rename_expr ρ used0 arg in
+              let (rest', used2) := go used1 rest in
+              (arg' :: rest', used2)
+          end) used l) as r eqn:Hargs.
+    destruct r as [argsr used_args].
+    injection Hrename as <- _.
+    lazymatch goal with
+    | Htyped_call : typed fenvr Γr (ECall ?fname argsr) T Γr' |- _ =>
+      destruct (typed_call_inv fenvr Γr fname argsr T Γr' Htyped_call)
+        as [fdef [Hinr [Hname_r [Hret_r Hargs_typed]]]];
+      destruct (fenv_alpha_in_backward fenv0 fenvr fdef Hfenv Hinr)
+        as [fdef0 [Hin0 Hshape]];
+      destruct Hshape as [Hname [Hret Hparams]]
+    end.
+    assert (Hargs_back :
+      exists Γ0',
+        typed_args fenv0 Γ0 l (fn_params fdef0) Γ0' /\
+        ctx_alpha ρ Γ0' Γr').
+    { eapply alpha_rename_call_args_typed_backward.
+      - intros Γa Γb used0 e er used1 T0 Γb' Hin Halpha Hcu Hru Hd Hr Ht.
+        eapply IH.
+        + pose proof (expr_size_call_arg_lt i l e Hin) as Harg_lt.
+          eapply Nat.lt_le_trans.
+          * exact Harg_lt.
+          * simpl. simpl in Hlt. lia.
+        + exact Hfenv.
+        + exact Halpha.
+        + exact Hcu.
+        + exact Hru.
+        + exact Hd.
+        + exact Hr.
+        + exact Ht.
+      - exact Hfenv.
+      - exact Hctx.
+      - exact Hctx_used.
+      - exact Hrange_used.
+      - exact Hdisj.
+      - exact Hparams.
+      - symmetry. exact Hargs.
+      - lazymatch goal with
+        | Hargs_typed : typed_args fenvr Γr argsr _ Γr' |- _ => exact Hargs_typed
+        end. }
+    destruct Hargs_back as [Γ0' [Htyped_args0 Hctx0]].
+    exists Γ0'. split.
+    * rewrite <- Hret_r. rewrite <- Hret.
+      eapply T_Call.
+      -- exact Hin0.
+      -- rewrite Hname. exact Hname_r.
+      -- exact Htyped_args0.
+    * exact Hctx0.
+  + destruct p as [px].
+    destruct (alpha_rename_expr ρ used e) as [er0 used0] eqn:He.
+    injection Hrename as <- _.
+    inversion Htyped; subst.
+    assert (Hsafe : ~ In px (rename_range ρ)).
+    { intros Hin. apply (Hdisj px); simpl; [left; reflexivity | exact Hin]. }
+    assert (Hdisj_e : disjoint_names (free_vars_expr e) (rename_range ρ)).
+    { intros x Hin Hinr. exact (Hdisj x (or_intror Hin) Hinr). }
+    lazymatch goal with
+    | Hte : typed fenvr Γr er0 ?Tnew ?Γr1 |- _ =>
+      destruct (IH fenv0 fenvr ρ Γ0 Γr e er0 used used0 Tnew Γr1
+        ltac:(simpl in Hlt; lia)
+        Hfenv Hctx Hctx_used Hrange_used
+        Hdisj_e He Hte) as [Γ0' [Htyped0 Hctx0]]
+    end.
+    exists Γ0'. split.
+    { eapply T_Replace.
+      - lazymatch goal with
+        | Hlookup : ctx_lookup (lookup_rename px ρ) Γr = Some (?Tx, false) |- _ =>
+          exact (ctx_alpha_lookup_backward ρ Γ0 Γr px Tx false Hctx Hsafe Hlookup)
+        end.
+      - exact Htyped0.
+      - assumption.
+      - assumption. }
+    { exact Hctx0. }
+  + destruct (alpha_rename_expr ρ used e) as [er0 used0] eqn:He.
+    injection Hrename as <- _.
+    inversion Htyped; subst.
+    destruct (IH fenv0 fenvr ρ Γ0 Γr e er0 used used0 T0 Γr'
+      ltac:(simpl in Hlt; lia)
+      Hfenv Hctx Hctx_used Hrange_used Hdisj He H1)
+      as [Γ0' [Htyped0 Hctx0]].
+    exists Γ0'. split; [eapply T_Drop; exact Htyped0 | exact Hctx0].
+  }
+  intros fenv0 fenvr ρ Γ0 Γr e er used used' T Γr'
+    Hfenv Hctx Hctx_used Hrange_used Hdisj Hrename Htyped.
+  eapply (Hsize (S (expr_size e))).
+  - apply Nat.lt_succ_diag_r.
+  - exact Hfenv.
+  - exact Hctx.
+  - exact Hctx_used.
+  - exact Hrange_used.
+  - exact Hdisj.
+  - exact Hrename.
+  - exact Htyped.
+Qed.
 
 Lemma infer_call_args_sound : forall fenv Γ args params Γ',
   (forall Γ0 e T Γ1,
@@ -938,12 +1653,26 @@ Lemma alpha_rename_for_infer_typed_backward : forall fenv Γ e fenv' e' T Γ',
   typed fenv Γ e T Γ'.
 Proof.
   intros fenv Γ e fenv' e' T Γ' Hrename Htyped.
-  pose proof (alpha_rename_for_infer_sound
-    fenv Γ e fenv' e' Hrename) as [Hfenv_alpha Hexpr_alpha].
-  destruct typed_alpha_backward as [Htyped_backward _].
-  pose proof (Htyped_backward
-    fenv' Γ e' T Γ' Htyped
-    fenv [] Γ e Hfenv_alpha (CtxAlpha_Base Γ) Hexpr_alpha)
+  unfold alpha_rename_for_infer in Hrename.
+  destruct (alpha_rename_syntax_go (free_vars_expr e ++ ctx_names Γ) fenv)
+    as [fenv0 used] eqn:Hfenv.
+  destruct (alpha_rename_expr [] used e) as [er used'] eqn:He.
+  injection Hrename as <- <-.
+  pose proof (alpha_rename_syntax_go_shape
+    (free_vars_expr e ++ ctx_names Γ) fenv fenv0 used Hfenv) as Hfenv_alpha.
+  assert (Hctx_used : forall x, In x (ctx_names Γ) -> In x used).
+  { intros x Hin.
+    eapply alpha_rename_syntax_go_used_extends.
+    - exact Hfenv.
+    - apply in_or_app. right. exact Hin. }
+  assert (Hrange_used : forall x, In x (rename_range []) -> In x used).
+  { intros x Hin. contradiction. }
+  assert (Hdisj : disjoint_names (free_vars_expr e) (rename_range [])).
+  { apply disjoint_names_nil_r. }
+  pose proof (alpha_rename_typed_backward
+    fenv fenv0 [] Γ Γ e er used used' T Γ'
+    Hfenv_alpha (CtxAlpha_Base Γ)
+    Hctx_used Hrange_used Hdisj He Htyped)
     as [Γ0 [Htyped0 Hctx_alpha]].
   pose proof (ctx_alpha_nil_eq Γ0 Γ' Hctx_alpha) as Heq.
   subst Γ0.
